ml-dsa make

libcrux-ml-dsa/proofs/fstar/extraction/Libcrux_ml_dsa.Simd.Avx2.Encoding.Commitment.fst
@@ -3,30 +3,34 @@ module Libcrux_ml_dsa.Simd.Avx2.Encoding.Commitment
 open Core
 open FStar.Mul
 
-let serialize (v_OUTPUT_SIZE: usize) (simd_unit: u8) =
+let serialize (v_OUTPUT_SIZE: usize) (simd_unit: Libcrux_intrinsics.Avx2_extract.t_Vec256) =
   let serialized:t_Array u8 (sz 19) = Rust_primitives.Hax.repeat 0uy (sz 19) in
   match cast (v_OUTPUT_SIZE <: usize) <: u8 with
   | 4uy ->
-    let adjacent_2_combined:u8 =
+    let adjacent_2_combined:Libcrux_intrinsics.Avx2_extract.t_Vec256 =
       Libcrux_intrinsics.Avx2_extract.mm256_sllv_epi32 simd_unit
-        (Libcrux_intrinsics.Avx2_extract.mm256_set_epi32 0l 28l 0l 28l 0l 28l 0l 28l <: u8)
+        (Libcrux_intrinsics.Avx2_extract.mm256_set_epi32 0l 28l 0l 28l 0l 28l 0l 28l
+          <:
+          Libcrux_intrinsics.Avx2_extract.t_Vec256)
     in
-    let adjacent_2_combined:u8 =
+    let adjacent_2_combined:Libcrux_intrinsics.Avx2_extract.t_Vec256 =
       Libcrux_intrinsics.Avx2_extract.mm256_srli_epi64 28l adjacent_2_combined
     in
-    let adjacent_4_combined:u8 =
+    let adjacent_4_combined:Libcrux_intrinsics.Avx2_extract.t_Vec256 =
       Libcrux_intrinsics.Avx2_extract.mm256_permutevar8x32_epi32 adjacent_2_combined
-        (Libcrux_intrinsics.Avx2_extract.mm256_set_epi32 0l 0l 0l 0l 6l 2l 4l 0l <: u8)
+        (Libcrux_intrinsics.Avx2_extract.mm256_set_epi32 0l 0l 0l 0l 6l 2l 4l 0l
+          <:
+          Libcrux_intrinsics.Avx2_extract.t_Vec256)
     in
-    let adjacent_4_combined:u8 =
+    let adjacent_4_combined:Libcrux_intrinsics.Avx2_extract.t_Vec128 =
       Libcrux_intrinsics.Avx2_extract.mm256_castsi256_si128 adjacent_4_combined
     in
-    let adjacent_4_combined:u8 =
+    let adjacent_4_combined:Libcrux_intrinsics.Avx2_extract.t_Vec128 =
       Libcrux_intrinsics.Avx2_extract.mm_shuffle_epi8 adjacent_4_combined
         (Libcrux_intrinsics.Avx2_extract.mm_set_epi8 240uy 240uy 240uy 240uy 240uy 240uy 240uy 240uy
             240uy 240uy 240uy 240uy 12uy 4uy 8uy 0uy
           <:
-          u8)
+          Libcrux_intrinsics.Avx2_extract.t_Vec128)
     in
     let serialized:t_Array u8 (sz 19) =
       Rust_primitives.Hax.Monomorphized_update_at.update_at_range serialized
@@ -58,33 +62,39 @@ let serialize (v_OUTPUT_SIZE: usize) (simd_unit: u8) =
         <:
         Core.Result.t_Result (t_Array u8 v_OUTPUT_SIZE) Core.Array.t_TryFromSliceError)
   | 6uy ->
-    let adjacent_2_combined:u8 =
+    let adjacent_2_combined:Libcrux_intrinsics.Avx2_extract.t_Vec256 =
       Libcrux_intrinsics.Avx2_extract.mm256_sllv_epi32 simd_unit
-        (Libcrux_intrinsics.Avx2_extract.mm256_set_epi32 0l 26l 0l 26l 0l 26l 0l 26l <: u8)
+        (Libcrux_intrinsics.Avx2_extract.mm256_set_epi32 0l 26l 0l 26l 0l 26l 0l 26l
+          <:
+          Libcrux_intrinsics.Avx2_extract.t_Vec256)
     in
-    let adjacent_2_combined:u8 =
+    let adjacent_2_combined:Libcrux_intrinsics.Avx2_extract.t_Vec256 =
       Libcrux_intrinsics.Avx2_extract.mm256_srli_epi64 26l adjacent_2_combined
     in
-    let adjacent_3_combined:u8 =
+    let adjacent_3_combined:Libcrux_intrinsics.Avx2_extract.t_Vec256 =
       Libcrux_intrinsics.Avx2_extract.mm256_shuffle_epi8 adjacent_2_combined
         (Libcrux_intrinsics.Avx2_extract.mm256_set_epi8 (-1y) (-1y) (-1y) (-1y) (-1y) (-1y) (-1y)
             (-1y) (-1y) (-1y) (-1y) (-1y) 9y 8y 1y 0y (-1y) (-1y) (-1y) (-1y) (-1y) (-1y) (-1y)
             (-1y) (-1y) (-1y) (-1y) (-1y) 9y 8y 1y 0y
           <:
-          u8)
+          Libcrux_intrinsics.Avx2_extract.t_Vec256)
     in
-    let adjacent_3_combined:u8 =
+    let adjacent_3_combined:Libcrux_intrinsics.Avx2_extract.t_Vec256 =
       Libcrux_intrinsics.Avx2_extract.mm256_mullo_epi16 adjacent_3_combined
         (Libcrux_intrinsics.Avx2_extract.mm256_set_epi16 1s 1s 1s 1s 1s 1s 1s (1s <<! 4l <: i16) 1s
             1s 1s 1s 1s 1s 1s (1s <<! 4l <: i16)
           <:
-          u8)
+          Libcrux_intrinsics.Avx2_extract.t_Vec256)
     in
-    let adjacent_3_combined:u8 =
+    let adjacent_3_combined:Libcrux_intrinsics.Avx2_extract.t_Vec256 =
       Libcrux_intrinsics.Avx2_extract.mm256_srlv_epi32 adjacent_3_combined
-        (Libcrux_intrinsics.Avx2_extract.mm256_set_epi32 0l 0l 0l 4l 0l 0l 0l 4l <: u8)
+        (Libcrux_intrinsics.Avx2_extract.mm256_set_epi32 0l 0l 0l 4l 0l 0l 0l 4l
+          <:
+          Libcrux_intrinsics.Avx2_extract.t_Vec256)
     in
-    let lower_3_:u8 = Libcrux_intrinsics.Avx2_extract.mm256_castsi256_si128 adjacent_3_combined in
+    let lower_3_:Libcrux_intrinsics.Avx2_extract.t_Vec128 =
+      Libcrux_intrinsics.Avx2_extract.mm256_castsi256_si128 adjacent_3_combined
+    in
     let serialized:t_Array u8 (sz 19) =
       Rust_primitives.Hax.Monomorphized_update_at.update_at_range serialized
         ({ Core.Ops.Range.f_start = sz 0; Core.Ops.Range.f_end = sz 16 }
@@ -102,7 +112,7 @@ let serialize (v_OUTPUT_SIZE: usize) (simd_unit: u8) =
           <:
           t_Slice u8)
     in
-    let upper_3_:u8 =
+    let upper_3_:Libcrux_intrinsics.Avx2_extract.t_Vec128 =
       Libcrux_intrinsics.Avx2_extract.mm256_extracti128_si256 1l adjacent_3_combined
     in
     let serialized:t_Array u8 (sz 19) =
