libcrux-ml-dsa/proofs/fstar/extraction/Libcrux_ml_dsa.Simd.Avx2.Encoding.Gamma1.fsti
@@ -18,19 +18,23 @@ let serialize_when_gamma1_is_2_pow_17___GAMMA1: i32 = 1l <<! 17l
 let serialize_when_gamma1_is_2_pow_19___GAMMA1: i32 = 1l <<! 19l
 
 val deserialize_when_gamma1_is_2_pow_17_ (serialized: t_Slice u8)
-    : Prims.Pure u8 Prims.l_True (fun _ -> Prims.l_True)
+    : Prims.Pure Libcrux_intrinsics.Avx2_extract.t_Vec256 Prims.l_True (fun _ -> Prims.l_True)
 
 val deserialize_when_gamma1_is_2_pow_19_ (serialized: t_Slice u8)
-    : Prims.Pure u8 Prims.l_True (fun _ -> Prims.l_True)
+    : Prims.Pure Libcrux_intrinsics.Avx2_extract.t_Vec256 Prims.l_True (fun _ -> Prims.l_True)
 
 val deserialize (v_GAMMA1_EXPONENT: usize) (serialized: t_Slice u8)
-    : Prims.Pure u8 Prims.l_True (fun _ -> Prims.l_True)
+    : Prims.Pure Libcrux_intrinsics.Avx2_extract.t_Vec256 Prims.l_True (fun _ -> Prims.l_True)
 
-val serialize_when_gamma1_is_2_pow_17_ (v_OUTPUT_SIZE: usize) (simd_unit: u8)
+val serialize_when_gamma1_is_2_pow_17_
+      (v_OUTPUT_SIZE: usize)
+      (simd_unit: Libcrux_intrinsics.Avx2_extract.t_Vec256)
     : Prims.Pure (t_Array u8 v_OUTPUT_SIZE) Prims.l_True (fun _ -> Prims.l_True)
 
-val serialize_when_gamma1_is_2_pow_19_ (v_OUTPUT_SIZE: usize) (simd_unit: u8)
+val serialize_when_gamma1_is_2_pow_19_
+      (v_OUTPUT_SIZE: usize)
+      (simd_unit: Libcrux_intrinsics.Avx2_extract.t_Vec256)
     : Prims.Pure (t_Array u8 v_OUTPUT_SIZE) Prims.l_True (fun _ -> Prims.l_True)
 
-val serialize (v_OUTPUT_SIZE: usize) (simd_unit: u8)
+val serialize (v_OUTPUT_SIZE: usize) (simd_unit: Libcrux_intrinsics.Avx2_extract.t_Vec256)
     : Prims.Pure (t_Array u8 v_OUTPUT_SIZE) Prims.l_True (fun _ -> Prims.l_True)
